Test/dafny0/RefinementErrors.dfy
@@ -4,6 +4,19 @@ module A {
     {
       x := 6;
     }
+
+    var abc: bool;
+    var xyz: bool;
+
+    function method F<A,B,C>(x: int, y: A, z: set<C>, b: bool): B
+
+    function G(): int  // uninterpreted for now
+    function H(): int  // uninterpreted for now
+
+    method BodyLess(y: bool, k: seq<set<object>>) returns (x: int)
+    method FullBodied(x: int) returns (y: bool, k: seq<set<object>>)
+    {
+    }
   }
 }
 
@@ -14,5 +27,32 @@ module B refines A {
       requires 0 <= y;  // error: cannot add a precondition
       modifies this;  // error: cannot add a modifies clause
       ensures 0 <= x;  // fine
+
+    predicate abc  // error: cannot replace a field with a predicate
+    var xyz: bool;  // error: ...or even with another field
+
+    function F   // error: cannot replace a "function method" with a "function"
+        <C,A,B>  // error: different list of type parameters
+        (x: int, y: A, z: seq<C>,  // error: different type of parameter z
+         k: bool)  // error: different parameter name
+        : B
+
+    function G(): int
+    { 12 }  // allowed to add a body
+
+    method BodyLess(y: bool, k: seq<set<object>>) returns (x: int)
+    {  // yes, can give it a body
+    }
+    method FullBodied(x: int) returns (y: bool, k: seq<set<object>>)
+    {  // error: not allowed to change body (not yet implemented)
+    }
+  }
+}
+
+module BB refines B {
+  class C {
+    function method G(): int  // error: allowed to make a function into a function method
+    function method H(): int  // ...unless this is where the function body is given
+    { 10 }
   }
 }
